Rocq/src/Context.v
@@ -1,0 +1,151 @@
+From Stdlib Require Import Lists.List.
+From Verilog Require Import Expr.
+From Verilog Require Import Path.
+From Verilog Require Import Utils.
+
+Import ListNotations.
+Import Expr.
+Import Path.
+Import Utils.
+
+Import Notation.
+
+Set Implicit Arguments.
+
+Definition push {X: Type} l (x: X) := l ++ [x].
+
+Fixpoint e_ctx (e: Expr) (p: path) : list path :=
+  match e with
+  | EOperand _ => []
+  | EBinOp lhs rhs => e_ctx lhs (push p Lhs) ++ e_ctx rhs (push p Rhs)
+  | EUnOp arg => e_ctx arg (push p Arg)
+  | ECast arg => let p' := push p Arg in p' :: e_ctx arg p'
+  | EComp lhs rhs => p :: e_ctx lhs (push p Lhs) ++ e_ctx rhs (push p Rhs)
+  | ELogic lhs rhs =>
+      let lhsP := push p Lhs in
+      let rhsP := push p Rhs in
+      lhsP :: e_ctx lhs lhsP ++ rhsP :: e_ctx rhs rhsP
+  | EReduction arg => let p' := push p Arg in p' :: e_ctx arg p'
+  | EShift lhs rhs =>
+      let rhsP := push p Rhs in
+      e_ctx lhs (push p Lhs) ++ rhsP :: e_ctx rhs rhsP
+  | EAssign _ arg => let p' := push p Arg in p' :: e_ctx arg p'
+  | EShiftAssign _ arg => let p' := push p Arg in p' :: e_ctx arg p'
+  | ECond cond tb fb =>
+      let condP := push p Cond in
+      condP :: e_ctx cond condP ++ e_ctx tb (push p TrueB)
+        ++ e_ctx fb (push p FalseB)
+  | EConcat args =>
+      concat (mapI (fun i e => let newP := push p (Args i) in newP :: e_ctx e newP) args)
+  | ERepl _ arg => let p' := push p Arg in p' :: e_ctx arg p'
+  | EInside arg args =>
+      concat (mapI (fun i e => let newP := push p (Args i) in newP :: e_ctx e newP) args)
+  end
+.
+
+Definition contexts (e: Expr) := [] :: e_ctx e [].
+
+Lemma e_ctx_comp: forall e p c, In c (e_ctx e p) -> exists l, c = p ++ l /\ IsPath e l.
+Proof.
+  Ltac _e_ctx_comp_tac :=
+    match goal with
+    | [ H: ex _ |- ex _ ] =>
+        destruct H as [? [H1 H2]]; subst; eexists; split;
+        [ rewrite <- app_assoc; reflexivity | constructor; assumption]
+    | [ IHe: _, H : In _ (e_ctx _ _) |- _ ] =>
+        apply IHe in H; _e_ctx_comp_tac
+    | [ H : In _ (_ :: e_ctx _ _) |- _ ] =>
+        apply in_inv in H; destruct H; subst; _e_ctx_comp_tac
+    | [ IHe: _, H: In _ (concat _) |- _ ] =>
+        apply in_concat in H; destruct H as [x [H H2]]; apply mapI_values in H;
+        destruct H as [n [x0 [H1 H3]]]; subst; apply in_inv in H2; destruct H2; subst;
+        [ exists [Args n]; split; [reflexivity | econstructor; [apply H1 | constructor]]
+        | destruct (IHe _ _ _ _ H1 H) as [? [H2 H3]]; subst; eexists; split;
+          [rewrite <- app_assoc; reflexivity | econstructor; [apply H1 | assumption]]]
+    | [ _ : _ |- ex (fun _ => _ ++ [?x] = _ /\ _) ] =>
+        exists [x]; split; [reflexivity | constructor; constructor]
+    end
+  .
+  induction e using Expr_ind with
+    (P0 := fun args => forall n e p c, nth_error args n = Some e -> In c (e_ctx e p)
+                               -> exists l, c = p ++ l /\ IsPath e l);
+    intros; simpl in *; unfold push in *;
+    repeat (rewrite in_app_iff in *; destruct H as [H|H]); intuition; subst;
+    try _e_ctx_comp_tac.
+  - exists []. rewrite app_nil_r. split. reflexivity. constructor.
+  - destruct n; discriminate H.
+  - destruct n; simpl in *.
+    + inv H. apply (IHe _ _ H0).
+    + apply (IHe0 _ _ _ _ H H0).
+Qed.
+
+
+Lemma e_ctx_prefix: forall e p c, In (p ++ c) (e_ctx e p) <-> In c (e_ctx e []).
+Proof.
+  Ltac _e_ctx_pre_tac_internal :=
+    match goal with
+    | [ IHe: _, _: In (_ ++ _) _ |- _ ] =>
+        rewrite app_assoc in *; rewrite IHe in *; intuition
+    end
+  .
+  Ltac _e_ctx_pre_tac :=
+    match goal with
+    | [ H: In _ (e_ctx _ [_]) |- _ ] =>
+        destruct (e_ctx_comp _ _ _ H) as [? [? _]]; subst; _e_ctx_pre_tac_internal
+    | [ H: In _ (e_ctx _ (_ ++ _)) |- _ ] =>
+        destruct (e_ctx_comp _ _ _ H) as [? [?He _]]; rewrite <- app_assoc in He;
+        apply app_inv_head in He; subst; _e_ctx_pre_tac_internal
+    | [ H: ?x ++ _ = ?x ++ _ |- _ ] => apply app_inv_head in H; subst; intuition
+    end
+  .
+  induction e using Expr_ind with
+    (P0 := fun args => forall n e p c, nth_error args n = Some e ->
+                               In (p ++ c) (e_ctx e p) <-> In c (e_ctx e []));
+    intros; simpl in *; unfold push in *; repeat (rewrite in_app_iff); simpl in *;
+    split; intros H0; intuition; try _e_ctx_pre_tac; subst; auto.
+  - left. apply (app_inv_head p). rewrite app_nil_r. assumption.
+  - left. symmetry. apply app_nil_r.
+  - rewrite in_concat in *. destruct H0 as [x [H1 H2]]. rewrite mapI_values in H1.
+    destruct H1 as [n [e [H1 H3]]]. subst. simpl in H2. destruct H2; eexists;
+      rewrite mapI_values; split; try (exists n; exists e; split; [apply H1 | reflexivity]).
+    + left. apply (app_inv_head p). assumption.
+    + right. _e_ctx_pre_tac. apply H1. apply H1.
+  - rewrite in_concat in *. destruct H0 as [x [H1 H2]]. rewrite mapI_values in H1.
+    destruct H1 as [n [e [H1 H3]]]. subst. simpl in H2. destruct H2; eexists;
+      rewrite mapI_values; split; try (exists n; exists e; split; [apply H1 | reflexivity]).
+    + subst. left. reflexivity.
+    + right. _e_ctx_pre_tac. apply H1. apply H1.
+  - rewrite in_concat in *. destruct H0 as [x [H1 H2]]. rewrite mapI_values in H1.
+    destruct H1 as [n [f [H1 H3]]]. subst. simpl in H2. destruct H2; eexists;
+      rewrite mapI_values; split; try (exists n; exists f; split; [apply H1 | reflexivity]).
+    + left. apply (app_inv_head p). assumption.
+    + right. _e_ctx_pre_tac. apply H1. apply H1.
+  - rewrite in_concat in *. destruct H0 as [x [H1 H2]]. rewrite mapI_values in H1.
+    destruct H1 as [n [f [H1 H3]]]. subst. simpl in H2. destruct H2; eexists;
+      rewrite mapI_values; split; try (exists n; exists f; split; [apply H1 | reflexivity]).
+    + subst. left. reflexivity.
+    + right. _e_ctx_pre_tac. apply H1. apply H1.
+  - destruct n; discriminate H.
+  - destruct n; discriminate H.
+  - destruct n. inv H. firstorder. simpl in H. eapply (IHe0 _ _ _ _ H). apply H0.
+  - destruct n. inv H. firstorder. simpl in H. eapply (IHe0 _ _ _ _ H). apply H0.
+Qed.
+
+Lemma e_ctx_is_path: forall e e0 p c,
+    sub_expr e p = Some e0 -> In c (e_ctx e0 p) -> IsPath e c.
+Proof.
+  intros e e0 p c H1 H2.
+  assert (H3: exists l, c = p ++ l /\ IsPath e0 l). apply (e_ctx_comp _ _ _ H2).
+  destruct H3 as [l [H3 H4]].
+  apply IsPath_chunk. exists p. exists e0. exists l. intuition.
+Search IsPath.
+Qed.
+
+
+Lemma contexts_is_path: forall e c, In c (contexts e) -> IsPath e c.
+Proof.
+  intros. unfold contexts in H. simpl in H. destruct H.
+  - subst. constructor.
+  - apply (e_ctx_is_path _ _ _ (sub_exp_nil e) H).
+Qed.
+
