Rocq/src/Path.v
@@ -1,0 +1,301 @@
+From Stdlib Require Import Lists.List.
+From Stdlib Require Arith.Arith.
+From Verilog Require Import Expr.
+From Verilog Require Import Utils.
+
+Import ListNotations.
+Import Expr.
+Import Utils.
+
+Set Implicit Arguments.
+
+Module Path.
+  Inductive PathItem :=
+  | Lhs
+  | Rhs
+  | Arg
+  | Cond
+  | TrueB
+  | FalseB
+  | Args (i: nat)
+  .
+
+  Definition path : Type := list PathItem.
+
+  Inductive IsPath : Expr -> path -> Prop :=
+  | P_Empty : forall e, IsPath e []
+  | P_LhsBinOp : forall lhs rhs p, IsPath lhs p -> IsPath (EBinOp lhs rhs) (Lhs :: p)
+  | P_RhsBinOp : forall lhs rhs p, IsPath rhs p -> IsPath (EBinOp lhs rhs) (Rhs :: p)
+  | P_UnOpArg : forall arg p, IsPath arg p -> IsPath (EUnOp arg) (Arg :: p)
+  | P_CastArg : forall arg p, IsPath arg p -> IsPath (ECast arg) (Arg :: p)
+  | P_LhsCompOp : forall lhs rhs p, IsPath lhs p -> IsPath (EComp lhs rhs) (Lhs :: p)
+  | P_RhsCompOp : forall lhs rhs p, IsPath rhs p -> IsPath (EComp lhs rhs) (Rhs :: p)
+  | P_LhsLogic : forall lhs rhs p, IsPath lhs p -> IsPath (ELogic lhs rhs) (Lhs :: p)
+  | P_RhsLogic : forall lhs rhs p, IsPath rhs p -> IsPath (ELogic lhs rhs) (Rhs :: p)
+  | P_RedArg : forall arg p, IsPath arg p -> IsPath (EReduction arg) (Arg :: p)
+  | P_LhsShift : forall lhs rhs p, IsPath lhs p -> IsPath (EShift lhs rhs) (Lhs :: p)
+  | P_RhsShift : forall lhs rhs p, IsPath rhs p -> IsPath (EShift lhs rhs) (Rhs :: p)
+  | P_AssignArg : forall op arg p, IsPath arg p -> IsPath (EAssign op arg) (Arg :: p)
+  | P_ShiftAssignArg : forall op arg p, IsPath arg p -> IsPath (EShiftAssign op arg) (Arg :: p)
+  | P_CondCond : forall cond tb fb p, IsPath cond p -> IsPath (ECond cond tb fb) (Cond :: p)
+  | P_CondTrue : forall cond tb fb p, IsPath tb p -> IsPath (ECond cond tb fb) (TrueB :: p)
+  | P_CondFalse : forall cond tb fb p, IsPath fb p -> IsPath (ECond cond tb fb) (FalseB :: p)
+  | P_ConcatArgs : forall n args e p,
+      nth_error args n = Some e -> IsPath e p -> IsPath (EConcat args) (Args n :: p)
+  | P_ReplArg : forall i arg p, IsPath arg p -> IsPath (ERepl i arg) (Arg :: p)
+  | P_InsideArg : forall arg eList p, IsPath arg p -> IsPath (EInside arg eList) (Arg :: p)
+  | P_InsideRange : forall n arg eList e p,
+      nth_error eList n = Some e -> IsPath e p -> IsPath (EInside arg eList) (Args n :: p)
+  .
+
+
+  Lemma ispath_prefix: forall e p, IsPath e p -> forall l1 l2, l1 ++ l2 = p -> IsPath e l1.
+  Proof.
+    intros e p H. induction H; intros; try (destruct l1;
+      [constructor | inversion H0; constructor; firstorder]).
+    - apply app_eq_nil in H. intuition (subst; constructor).
+    - destruct l1.
+      + constructor.
+      + inversion H1. subst. clear H1. econstructor.
+        * apply H.
+        * apply (IHIsPath l1 l2). reflexivity.
+    - destruct l1.
+      + constructor.
+      + inversion H1. subst. clear H1. econstructor.
+        * apply H.
+        * apply (IHIsPath l1 l2). reflexivity.
+  Qed.
+
+  Definition add_path {X: Type} (x: X) := map (fun l => x :: l).
+
+  Lemma add_path_okay : forall (X: Type) (x: X) suf l,
+    In l (add_path x suf) <-> exists p, l = x :: p /\ In p suf.
+  Proof.
+    induction suf. intros.
+    - split; intros. contradiction. destruct H as [p [_ []]].
+    - split; intros.
+      + destruct H.
+        * subst. exists a. firstorder.
+        * rewrite IHsuf in H. destruct H as [p [H1 H2]]. exists p. firstorder.
+      + destruct H as [p [H1 H2]]. destruct H2; subst.
+        * left. reflexivity.
+        * right. apply IHsuf. exists p. firstorder.
+  Qed.
+
+  Fixpoint all_path e :=
+    match e with
+    | EOperand _ => [[]]
+    | EBinOp lhs rhs => [] :: add_path Lhs (all_path lhs) ++ add_path Rhs (all_path rhs)
+    | EUnOp arg => [] :: add_path Arg (all_path arg)
+    | ECast arg => [] :: add_path Arg (all_path arg)
+    | EComp lhs rhs => [] :: add_path Lhs (all_path lhs) ++ add_path Rhs (all_path rhs)
+    | ELogic lhs rhs => [] :: add_path Lhs (all_path lhs) ++ add_path Rhs (all_path rhs)
+    | EReduction arg => [] :: add_path Arg (all_path arg)
+    | EShift lhs rhs => [] :: add_path Lhs (all_path lhs) ++ add_path Rhs (all_path rhs)
+    | EAssign _ arg => [] :: add_path Arg (all_path arg)
+    | EShiftAssign _ arg => [] :: add_path Arg (all_path arg)
+    | ECond cond tb fb =>
+        [] :: add_path Cond (all_path cond) ++ add_path TrueB (all_path tb)
+          ++ add_path FalseB (all_path fb)
+    | EConcat args =>
+        let lPath := mapI (fun i e => add_path (Args i) (all_path e)) args in
+        [] :: concat lPath
+    | ERepl _ arg => [] :: add_path Arg (all_path arg)
+    | EInside arg l =>
+        let lPath := mapI (fun i e => add_path (Args i) (all_path e)) l in
+        [] :: add_path Arg (all_path arg) ++ concat lPath
+    end
+  .
+
+  Lemma all_path_valid : forall e p, In p (all_path e) <-> IsPath e p.
+  Proof.
+    Ltac UnBinTriOp :=
+      match goal with
+      | [ H : In _ (all_path (_ _ _ _)) |- _ ] =>
+          destruct H;
+          [ subst; constructor
+          | repeat (rewrite in_app_iff in H); repeat (rewrite add_path_okay in H);
+            destruct H as [[p' [H1 H2]]|[[p' [H1 H2]]|[p' [H1 H2]]]];
+            subst; constructor; firstorder
+          ]
+      | [ H: IsPath (_ _ _ _) _ |- _ ] =>
+          inversion H; subst; try (constructor; reflexivity);
+          right; repeat (rewrite in_app_iff); repeat (rewrite add_path_okay);
+          [left | right; left | right; right]; eexists; intuition; firstorder
+      | [ H : In _ (all_path (_ _ _)) |- _ ] =>
+          destruct H;
+          [ subst; constructor
+          | repeat (rewrite in_app_iff in H); repeat (rewrite add_path_okay in H);
+            destruct H as [[p' [H1 H2]]|[p' [H1 H2]]];
+            subst; constructor; firstorder
+          ]
+      | [ H: IsPath (_ _ _) _ |- _ ] =>
+          inversion H; subst; try (constructor; reflexivity);
+          right; repeat (rewrite in_app_iff); repeat (rewrite add_path_okay);
+          [left | right]; eexists; intuition; firstorder
+      | [ H: In _ (all_path (_ _)) |- _ ] =>
+          destruct H;
+          [ subst; constructor
+          | repeat (rewrite in_app_iff in H); repeat (rewrite add_path_okay in H);
+            destruct H as [p' [H1 H2]];
+            subst; constructor; firstorder
+          ]
+      | [ H: IsPath (_ _) _ |- _ ] =>
+          inversion H; subst; try (constructor; reflexivity);
+          right; repeat (rewrite in_app_iff); repeat (rewrite add_path_okay);
+          eexists; intuition; firstorder
+      end.
+    intro e.
+    induction e using Expr_ind with
+      (P0 := fun r => forall n e, nth_error r n = Some e -> forall p, In p (all_path e) <-> IsPath e p);
+      intros; try (split; intros; UnBinTriOp).
+    - split; intros.
+      + destruct H. subst. constructor. destruct H.
+      + inversion H. left. reflexivity.
+    - split; intros.
+      + destruct H; subst; try constructor.
+        rewrite in_concat in H. destruct H as [h [H1 H2]].
+        rewrite mapI_values in H1. destruct H1 as [n [x [H1 H3]]].
+        subst. rewrite add_path_okay in H2. destruct H2 as [p' [H2 H3]]. subst.
+        econstructor. apply H1. firstorder.
+      + inversion H.
+        * constructor. reflexivity.
+        * subst. right. rewrite in_concat. apply (IHe n e H1) in H2. eexists. split.
+          -- rewrite mapI_values. exists n. exists e. intuition.
+          -- rewrite add_path_okay. exists p0. intuition.
+    - split; intros.
+      + destruct H; subst; try constructor. rewrite in_app_iff in *. destruct H.
+        * rewrite add_path_okay in H. destruct H as [p' [H1 H2]].
+          subst. constructor. firstorder.
+        * rewrite in_concat in H. destruct H as [h [H1 H2]].
+          rewrite mapI_values in H1. destruct H1 as [n [x [H1 H3]]].
+          subst. rewrite add_path_okay in H2. destruct H2 as [p' [H2 H3]]. subst.
+          econstructor. apply H1. firstorder.
+      + inversion H.
+        * constructor. reflexivity.
+        * subst. simpl. right. rewrite in_app_iff. left. rewrite add_path_okay.
+          exists p0. intuition. firstorder.
+        * subst. simpl. right. rewrite in_app_iff. right. rewrite in_concat.
+          apply (IHe0 n e0 H2) in H4. eexists. split.
+          -- rewrite mapI_values. exists n. exists e0. intuition.
+          -- rewrite add_path_okay. exists p0. intuition.
+    - destruct n; discriminate H.
+    - destruct n.
+      + inversion H. subst. apply IHe.
+      + simpl in H. firstorder.
+  Qed.
+
+
+  Fixpoint sub_expr (e: Expr) (p: path) :=
+    match e, p with
+    | e, [] => Some e
+    | EBinOp lhs _, Lhs :: p => sub_expr lhs p
+    | EBinOp _ rhs, Rhs :: p => sub_expr rhs p
+    | EUnOp arg, Arg :: p => sub_expr arg p
+    | ECast arg, Arg :: p => sub_expr arg p
+    | EComp lhs _, Lhs :: p => sub_expr lhs p
+    | EComp _ rhs, Rhs :: p => sub_expr rhs p
+    | ELogic lhs _, Lhs :: p => sub_expr lhs p
+    | ELogic _ rhs, Rhs :: p => sub_expr rhs p
+    | EReduction arg, Arg :: p => sub_expr arg p
+    | EShift lhs _, Lhs :: p => sub_expr lhs p
+    | EShift _ rhs, Rhs :: p => sub_expr rhs p
+    | EAssign _ arg, Arg :: p => sub_expr arg p
+    | EShiftAssign _ arg, Arg :: p => sub_expr arg p
+    | ECond cond _ _, Cond :: p => sub_expr cond p
+    | ECond _ tb _, TrueB :: p => sub_expr tb p
+    | ECond _ _ fb, FalseB :: p => sub_expr fb p
+    | EConcat args, Args i :: p =>
+        match nth_error args i with
+        | Some e => sub_expr e p
+        | None => None
+        end
+    | ERepl _ arg, Arg :: p => sub_expr arg p
+    | EInside arg _, Arg :: p => sub_expr arg p
+    | EInside _ args, Args i :: p =>
+        match nth_error args i with
+        | Some e => sub_expr e p
+        | None => None
+        end
+    | _, _ :: _ => None
+    end
+  .
+
+  Lemma IsPath_is_sub_expr: forall e p, IsPath e p -> exists e0, sub_expr e p = Some e0.
+  Proof.
+    intros. induction H; try (destruct IHIsPath as [x H1]; exists x);
+      try (simpl; rewrite H); try (assumption). exists e. destruct e; reflexivity.
+  Qed.
+
+  Lemma sub_expr_valid: forall e p f, sub_expr e p = Some f -> IsPath e p.
+  Proof.
+    induction e using Expr_ind with
+      (P0 := fun r => forall n e, nth_error r n = Some e ->
+                          forall p f, sub_expr e p = Some f -> IsPath e p);
+        intros; try (destruct p as [|[]]; try (discriminate H); constructor; firstorder).
+      - destruct p as [|[]]; try (discriminate H).
+        + constructor.
+        + simpl in H. destruct (nth_error args i) eqn:H1; try (discriminate H).
+          econstructor. apply H1. apply (IHe _ _ H1 _ _ H).
+      - destruct p as [|[]]; try (discriminate H).
+        + constructor.
+        + constructor. firstorder.
+        + simpl in H. destruct (nth_error range i) eqn:H1; try (discriminate H).
+          econstructor. apply H1.  apply (IHe0 _ _ H1 _ _ H).
+      - destruct n; discriminate H.
+      - destruct n.
+        + inversion H. subst. apply (IHe _ _ H0).
+        + apply (IHe0 _ _ H _ _ H0).
+  Qed.
+
+  Lemma sub_exp_nil: forall e, sub_expr e [] = Some e.
+  Proof.
+    intros. destruct e; reflexivity.
+  Qed.
+
+  Lemma sub_exp_chunk : forall p q e g,
+      (exists f, sub_expr e p = Some f /\ sub_expr f q = Some g)
+      <-> sub_expr e (p ++ q) = Some g.
+  Proof.
+    induction p; split; intros.
+    - destruct H as [f [H1 H2]]. rewrite sub_exp_nil in H1. inv H1. assumption.
+    - exists e. split. apply sub_exp_nil. assumption.
+    - destruct H as [f [H1 H2]]. destruct e; simpl; try (discriminate H1);
+        destruct a; simpl in *; try (destruct (nth_error _ i));
+        (apply IHp; exists f; intuition) || discriminate H1.
+    - destruct a; simpl in H;
+        try (destruct e; discriminate H || (apply IHp in H; assumption));
+        destruct e; discriminate H || (destruct (nth_error _ i) eqn:H';
+        discriminate H || (apply IHp in H; simpl; rewrite H'; assumption)).
+  Qed.
+
+  Lemma IsPath_chunk : forall e c,
+      IsPath e c <-> exists p f l, sub_expr e p = Some f /\ IsPath f l /\ c = p ++ l.
+  Proof.
+    Ltac _is_path_chunk_tac :=
+      match goal with
+      | [ H: _ |- context[_ = Some ?x] ] => destruct x; reflexivity
+      | [ H: _ = Some ?x |- context[_ = Some ?x] ] =>
+          simpl; rewrite H; destruct x; reflexivity
+      | [ C: _ = ?p ++ [], Q: sub_expr _ _ = Some ?e |- IsPath _ _] =>
+          rewrite app_nil_r in C; subst; apply sub_expr_valid with (f := e); assumption
+      | [ C: _ = ?p ++ ?a :: _, H: forall _, _ = _ -> _ = _ -> _,
+            Q: sub_expr _ _ = Some _ |- IsPath _ _] =>
+          apply (H (p ++ [a]));
+          [ apply sub_exp_chunk; eexists; split; [apply Q | _is_path_chunk_tac]
+          | subst; rewrite <- app_assoc; reflexivity]
+      end
+    .
+    split; intros.
+    - assert (H1: exists f, sub_expr e c = Some f). apply IsPath_is_sub_expr. assumption.
+      destruct H1 as [f H1]. exists c. exists f. exists []. repeat split. assumption. constructor.
+      symmetry. apply app_nil_r.
+    - destruct H as [p [f [l [H1 [H2 H3]]]]].
+      generalize dependent p. induction H2; intros; _is_path_chunk_tac.
+  Qed.
+
+  Lemma IsPath_suffix: forall e e0 p c l,
+    IsPath e c -> c = p ++ l -> sub_expr e p = Some e0 -> IsPath e0 l.
+  Proof.
+  Admitted.
+End Path.
