Rocq/src/Utils.v
@@ -1,0 +1,43 @@
+From Stdlib Require Import Lists.List.
+From Stdlib Require Import Lia.
+
+Import ListNotations.
+
+Module Utils.
+
+  Ltac inv H := inversion H; clear H; subst.
+
+
+  Fixpoint mapI'{X Y: Type} f i (l: list X) : list Y :=
+    match l with
+    | [] => []
+    | hd :: tl => f i hd :: mapI' f (i + 1) tl
+    end
+  .
+
+  Definition mapI {X Y: Type} (f: nat -> X -> Y) := mapI' f 0.
+
+  Lemma mapI'_values : forall (X Y: Type) (f: nat -> X -> Y) (l: list X) y i,
+      In y (mapI' f i l) <-> exists n x, nth_error l n = Some x /\ y = f (i + n) x.
+  Proof.
+    induction l.
+    - split; intros. contradiction. destruct H as [[|n] [x [H1 H2]]]; discriminate H1.
+    - split; intros.
+      + destruct H as [H1 | H2].
+        * exists 0. exists a. intuition. assert (HNat: i + 0 = i). lia. rewrite HNat. auto.
+        * rewrite IHl in H2. destruct H2 as [n [x [H1 H2]]].
+          exists (1 + n). exists x. intuition. assert (HNat: i + (1 + n) = i + 1 + n). lia.
+          rewrite HNat. apply H2.
+      + destruct H as [n [x [H1 H2]]]. destruct n.
+        * inversion H1. subst. left. assert (HNat: i + 0 = i). lia. rewrite HNat. reflexivity.
+        * right. apply IHl. exists n. exists x. intuition. assert (HNat: i + 1 + n = i + S n). lia.
+          rewrite HNat. apply H2.
+  Qed.
+
+  Lemma mapI_values:  forall (X Y: Type) (f: nat -> X -> Y) (l: list X) y,
+      In y (mapI f l) <-> exists n x, nth_error l n = Some x /\ y = f n x.
+  Proof.
+    intros. unfold mapI.  apply mapI'_values.
+  Qed.
+
+End Utils.
